\subsection*{Useful Formulae and Theorems}
\begin{align*}
    \tag{Combination} \binom{n}{r} & = \frac{n!}{r! (n-r)!}                                         \\
    \tag{Geometric Series}
    \sum_{k = 0}^{n - 1} r^k            & = \left( \frac{1 - r^n}{1 - r} \right)                         \\
                                        & \text{or}                                                      \\
    \sum_{i = 0}^{\infty} r^{i}         & = \frac{1}{1 - r} \quad \text{with} \quad \left| r \right| < 1
    \label{eqn:geometric-series}
\end{align*}

\begin{equation*} \tag{Euler's formula}
    e^{i x}=\cos x+i \sin x
    \label{eqn:Euler}
\end{equation*}

\begin{equation*}
    \tag{Newton's Binomial formula}
    (a+b)^{n}=\sum_{k=0}^{n} \binom{n}{k} a^{n-k} b^{k}
    \label{eqn:nbf}
\end{equation*}

\begin{thm}[Young's inequality for products] \label{theorem: youngs}
    If $a \geq 0$ and $b \geq 0$ are nonnegative real numbers and if $p > 1$ and $q > 1$ are real numbers such that $\frac{1}{p} + \frac{1}{p} = 1$, then
    \[
        ab \leq \frac{a^p}{p} + \frac{b^q}{q}.
    \]
    Equality holds iff $a^p = b^q$.
\end{thm}